resuming progress
we now halt on bad to avoid having to match server and signing indices

signedDH/easycrypt/SignedDH.ec
@@ -123,10 +123,8 @@ module SignedDH (S : SigScheme) (H : RO) : UATPaKE = {
   }
 }.
 
-module B1 (S : SigScheme) (A : Adv_UATPaKE_RO) (O : CMA_Oracles) = {
+module B1 (A : Adv_UATPaKE_RO) (O : CMA_Oracles) = {
   var b_ror : bool
-
-  var forgery : (int * (pdh * pdh) * sig) option
 
   var n : int
   var m : int
@@ -149,12 +147,11 @@ module B1 (S : SigScheme) (A : Adv_UATPaKE_RO) (O : CMA_Oracles) = {
     proc gen(): pkey = {
       var pk;
 
+      m <- m + 1;
       pk <@ O.gen();
+      pk_map.[m] <- pk;
       if (has (fun i pk_i=> pk_i = pk /\ p_map.[i] = None) pk_map) {
         pk <- witness;
-      } else {
-        m <- m + 1;
-        pk_map.[m] <- pk;
       }
       
       return pk;
@@ -229,8 +226,8 @@ module B1 (S : SigScheme) (A : Adv_UATPaKE_RO) (O : CMA_Oracles) = {
         
         if (c \notin odflt fset0 r_map.[p_map.[i], i]) {
           (h, sig) <- c;
-          b <@ S.verify(st_i.`pk, (st_i.`epk, h), sig);
-          if (b) {
+          b <@ O.verify(i, (st_i.`epk, h), sig);
+          if (b = Some true) {
             k <@ RO.get(st_i.`epk, h, h ^ st_i.`esk);
             ko <- Some k;
           }
@@ -238,9 +235,6 @@ module B1 (S : SigScheme) (A : Adv_UATPaKE_RO) (O : CMA_Oracles) = {
               /\ i \notin xp
               /\ p_map.[i] <> None /\ 0 < oget p_map.[i] <= m /\ oget p_map.[i] \notin cr
               /\ ko <> None) {
-            if (forgery <> None) {
-              forgery <- Some (oget p_map.[i], (st_i.`epk, h), sig);
-            }
             if (b_ror) { k <$ dssk; ko <- Some k; }
             ich <- ich `|` fset1 i;
           }
@@ -256,8 +250,6 @@ module B1 (S : SigScheme) (A : Adv_UATPaKE_RO) (O : CMA_Oracles) = {
     var b';
 
     RO.init();
-
-    forgery <- None;
 
     m <- 0;
     n <- 0;
@@ -278,27 +270,20 @@ module B1 (S : SigScheme) (A : Adv_UATPaKE_RO) (O : CMA_Oracles) = {
     h_map <- empty;
 
     b' <@ A(Oracles).distinguish();
-    return oget forgery;
   }
 }.
 
-module B1_0 (S : SigScheme) (A : Adv_UATPaKE_RO) (O : CMA_Oracles) = {
+module B1_0 (A : Adv_UATPaKE_RO) (O : CMA_Oracles) = {
   proc forge() = {
-    var f;
-
     B1.b_ror <- false;
-    f <@ B1(S, A, O).forge();
-    return f;
+    B1(A, O).forge();
   }
 }.
 
-module B1_1 (S : SigScheme) (A : Adv_UATPaKE_RO) (O : CMA_Oracles) = {
+module B1_1 (A : Adv_UATPaKE_RO) (O : CMA_Oracles) = {
   proc forge() = {
-    var f;
-
     B1.b_ror <- true;
-    f <@ B1(S, A, O).forge();
-    return f;
+    B1(A, O).forge();
   }
 }.
 
@@ -492,21 +477,27 @@ declare module A <: Adv_UATPaKE_RO { -Exp_b, -SUFCMA, -RO, -B1, -B2, -S }.
 local module Game0_b = {
   include var Exp_b(SignedDH(S), RO, A) [-run]
 
+  var halt_bad: bool
+
   module Oracles = {
     proc gen(): pkey = {
       var pk, sk;
 
-      m <- m + 1;
-      (pk, sk) <@ S.keygen();
-      pk_map.[m] <- pk;
-      sk_map.[m] <- sk;
+      if (!halt_bad) {
+        m <- m + 1;
+        (pk, sk) <@ S.keygen();
+        pk_map.[m] <- pk;
+        sk_map.[m] <- sk;
+      } else {
+        pk <- witness;
+      }
       return pk;
     }
 
     proc corrupt(j: int): skey option = {
       var r <- None;
 
-      if (0 < j <= m) {
+      if (!halt_bad /\ 0 < j <= m) {
         r <- sk_map.[j];
         cr <- cr `|` fset1 j;
       }
@@ -516,7 +507,7 @@ local module Game0_b = {
     proc expose(i) = {
       var r <- None;
 
-      if (0 < i <= n /\ i \notin ich) {
+      if (!halt_bad /\ 0 < i <= n /\ i \notin ich) {
         xp <- xp `|` fset1 i;
         r <- c_map.[i];
       }
@@ -526,15 +517,19 @@ local module Game0_b = {
     proc init(pk: pkey): pdh = {
       var st, jo, x, c;
 
-      n <- n + 1;
-      x <$ dsk;
-      c <- g ^ x;
-      st <- {| pk = pk; epk = c; esk = x |};
-      c_map.[n] <- st;
-      jo <- find (fun _ pk_j=> pk_j = pk) pk_map;
-      if (jo is Some j) {
-        p_map.[n] <- j;
-        i_map.[n] <- c;
+      if (!halt_bad) {
+        n <- n + 1;
+        x <$ dsk;
+        c <- g ^ x;
+        st <- {| pk = pk; epk = c; esk = x |};
+        c_map.[n] <- st;
+        jo <- find (fun _ pk_j=> pk_j = pk) pk_map;
+        if (jo is Some j) {
+          p_map.[n] <- j;
+          i_map.[n] <- c;
+        }
+      } else {
+        c <- witness;
       }
       return c;
     }
@@ -543,7 +538,7 @@ local module Game0_b = {
       var k, c', io, sk_j, h, y, sig;
       var r <- None;
 
-      if (0 < j <= m) {
+      if (!halt_bad /\ 0 < j <= m) {
         sk_j <- oget sk_map.[j];
         y <$ dsk;
         h <- g ^ y;
@@ -570,7 +565,7 @@ local module Game0_b = {
       var st_i, k, h, sig, b;
       var ko <- None;
 
-      if (0 < i <= n /\ i \notin q) {
+      if (!halt_bad /\ 0 < i <= n /\ i \notin q) {
         st_i <- oget c_map.[i];
         q <- q `|` fset1 i;
         
@@ -593,7 +588,16 @@ local module Game0_b = {
       return ko;
     }
 
-    proc h = RO.get
+    proc h(x) = {
+      var r;
+
+      if (!halt_bad) {
+        r <@ RO.get(x);
+      } else {
+        r <- witness;
+      }
+      return r;
+    }
   }
 
   proc run(b) = {
@@ -601,6 +605,7 @@ local module Game0_b = {
 
     RO.init();
 
+    halt_bad <- false;
     b_ror <- b;
 
     m <- 0;
@@ -621,42 +626,13 @@ local module Game0_b = {
     c_map <- empty;
 
     b' <@ A(Oracles).distinguish();
-    return b';
+    return b' /\ !halt_bad;
   }
 }.
 
-local lemma Hop0 &m:
-  `|  Pr[Exp_b(SignedDH(S), RO, A).run(false) @ &m: res]
-    - Pr[Exp_b(SignedDH(S), RO, A).run(true ) @ &m: res] |
-  = `|  Pr[Game0_b.run(false) @ &m: res]
-      - Pr[Game0_b.run(true ) @ &m: res] |.
-proof.
-have ^ + -> - -> //:
-  forall b, Pr[Exp_b(SignedDH(S), RO, A).run(b) @ &m: res]
-          = Pr[Game0_b.run(b) @ &m: res].
-move=> b; byequiv (: ={glob A, glob S, arg} ==> ={res})=> //.
-proc.
-(* The calls are equivalent due to equality on a bunch of variables *)
-call (: ={glob Exp_b(SignedDH(S), RO)}); last first.
-(* The invariant holds initially and allows us to conclude *)
-+ by inline *; auto.
-(* The invariant is preserved by all oracles *)
-+ by proc; inline *; auto; call (: true); auto.
-+ by proc; inline *; auto.
-+ by proc; inline *; auto.
-+ by proc; inline *; sim; auto.
-+ proc; inline *; sp; if; auto.
-  sim; auto.
-  by call (: true); auto.
-+ proc; sp; if; auto; sp; if; auto.
-  inline {1} 1.
-  by sim; auto.
-+ conseq (: _ ==> ={glob RO, res})=> //.
-  by sim.
-qed.
-
 local module Game1_b = {
   include var Exp_b(SignedDH(S), RO, A) [-run]
+  include var Game0_b [-run]
 
   var bad_1: bool
   var bad_2: bool
@@ -665,22 +641,26 @@ local module Game1_b = {
     include Game0_b.Oracles [-gen]
 
     proc gen(): pkey = {
-      var pk, sk;
-  
-      (pk, sk) <@ S.keygen();
-      if (has (fun i st=> st.`pk = pk /\ p_map.[i] = None) c_map) {
-        bad_1 <- true;
-        (* Pen and paper says "Stop" *)
-        (* Here, we don't stop; we just don't actually register the key and move on *)
-        (* The only thing we care about is the rest of the proof,
-           where we want to rely on the fact that each client instance
-           has at most one intended honest partner
-        *)
-        pk <- witness;
-      } else {
+      var sk, pk;
+ 
+      if (!halt_bad) {
         m <- m + 1;
+        (pk, sk) <@ S.keygen();
         pk_map.[m] <- pk;
         sk_map.[m] <- sk;
+        if (has (fun i st=> st.`pk = pk /\ p_map.[i] = None) c_map) {
+          bad_1 <- true;
+          (* Pen and paper says "Stop"; we can't stop because our
+             reductions *must* be black-box. We execute the adversary,
+             we do not simulate them: so we can't interrupt them
+             either. This is where the infrastructure we added in Hop
+             0 comes in.
+          *)
+          halt_bad <- true;
+          pk <- witness;
+        }
+      } else {
+        pk <- witness;
       }
       
       return pk;
@@ -692,6 +672,7 @@ local module Game1_b = {
 
     RO.init();
 
+    halt_bad <- false;
     b_ror <- b;
 
     m <- 0;
@@ -715,100 +696,23 @@ local module Game1_b = {
     bad_2 <- false;
 
     b' <@ A(Oracles).distinguish();
-    return b';
+    return b' /\ !halt_bad;
   }
 }.
 
 local module Game2_b = {
   include var Exp_b(SignedDH(S), RO, A) [-run]
+  include var Game0_b [-run]
   include var Game1_b [-run]
 
   module Oracles = {
-    proc gen(): pkey = {
-      var pk, sk;
-
-      (pk, sk) <@ S.keygen();
-      if (has (fun i st=> st.`pk = pk /\ p_map.[i] = None) c_map) {
-        bad_1 <- true;
-        (* Here, we don't stop; we just don't actually register the key and move on *)
-        pk <- witness;
-      } else {
-        m <- m + 1;
-        pk_map.[m] <- pk;
-        sk_map.[m] <- sk;
-      }
-      
-      return pk;
-    }
-
-    proc corrupt(j: int): skey option = {
-      var r <- None;
-
-      if (0 < j <= m) {
-        r <- sk_map.[j];
-        cr <- cr `|` fset1 j;
-      }
-      return r;
-    }
-
-    proc expose(i) = {
-      var r <- None;
-
-      if (0 < i <= n /\ i \notin ich) {
-        xp <- xp `|` fset1 i;
-        r <- c_map.[i];
-      }
-      return r;
-    }
-
-    proc init(pk: pkey): pdh = {
-      var st, jo, c, x;
-
-      n <- n + 1;
-      x <$ dsk;
-      c <- g ^ x;
-      st <- {| pk = pk; epk = c; esk = x |};
-      c_map.[n] <- st;
-      jo <- find (fun _ pk_j=> pk_j = pk) pk_map;
-      if (jo is Some j) {
-        p_map.[n] <- j;
-        i_map.[n] <- c;
-      }
-      return c;
-    }
-
-    proc respond(j: int, c: pdh, ch: bool): (sskey * (pdh * sig)) option = {
-      var k, c', io, sk_j, h, y, sig;
-      var r <- None;
-
-      if (0 < j <= m) {
-        sk_j <- oget sk_map.[j];
-        y <$ dsk;
-        h <- g ^ y;
-        sig <@ S.sign(sk_j, (c, h));
-        c' <- (h, sig);
-        k <@ RO.get(c, h, c ^ y);
-        io <- find (fun i _=> p_map.[i] = Some j /\ i_map.[i] = Some c) c_map;
-        if (io is Some i) {
-          (*** Instead of initialising all of r_map to output the
-          empty set, we read undefined entries as the empty set
-          here. ***)
-          r_map.[Some j, i] <- (odflt fset0 r_map.[Some j, i]) `|` fset1 c';
-          if (ch /\ i \notin xp) {
-            if (b_ror) { k <$ dssk; }
-            ich <- ich `|` fset1 i;
-          }
-        }
-        r <- Some (k, c');
-      }
-      return r;
-    }
+    include Game1_b.Oracles [-receive]
 
     proc receive(i: int, c: pdh * sig, ch: bool): sskey option = {
       var st_i, k, h, sig, b;
       var ko <- None;
 
-      if (0 < i <= n /\ i \notin q) {
+      if (!halt_bad /\ 0 < i <= n /\ i \notin q) {
         st_i <- oget c_map.[i];
         q <- q `|` fset1 i;
         
@@ -824,15 +728,13 @@ local module Game2_b = {
               /\ p_map.[i] <> None /\ 0 < oget p_map.[i] <= m /\ oget p_map.[i] \notin cr
               /\ ko <> None) {
             bad_2 <- true;
+            halt_bad <- true;
             ko <- None;
-            ich <- ich `|` fset1 i;
           }
         }
       }
       return ko;
     }
-
-    proc h = RO.get
   }
 
   proc run(b) = {
@@ -840,6 +742,7 @@ local module Game2_b = {
 
     RO.init();
 
+    halt_bad <- false;
     b_ror <- b;
 
     m <- 0;
@@ -863,7 +766,7 @@ local module Game2_b = {
     bad_2 <- false;
 
     b' <@ A(Oracles).distinguish();
-    return b';
+    return b' /\ !halt_bad;
   }
 }.
 
@@ -871,6 +774,46 @@ local module Game2_b = {
     in the sequence. We sometimes introduce intermediate modules as
     proof artefacts to enable formal reasoning.
 **)
+
+(* Hop 0: The distance between Game0(false) and Game0(true) is exactly
+          the advantage of A in distinguishing the real and ideal
+          experiments
+*)
+local lemma Hop0 &m:
+  `|  Pr[Exp_b(SignedDH(S), RO, A).run(false) @ &m: res]
+    - Pr[Exp_b(SignedDH(S), RO, A).run(true ) @ &m: res] |
+  = `|  Pr[Game0_b.run(false) @ &m: res]
+      - Pr[Game0_b.run(true ) @ &m: res] |.
+proof.
+have ^ + -> - -> //:
+  forall b, Pr[Exp_b(SignedDH(S), RO, A).run(b) @ &m: res]
+          = Pr[Game0_b.run(b) @ &m: res].
+move=> b; byequiv (: ={glob A, glob S, arg} ==> ={res})=> //.
+proc.
+(* The calls are equivalent due to equality on a bunch of variables *)
+call (: ={glob Exp_b(SignedDH(S), RO)} /\ !Game0_b.halt_bad{2}); last first.
+(* The invariant holds initially and allows us to conclude *)
++ by inline *; auto.
+(* The invariant is preserved by all oracles *)
++ proc; rcondt {2} ^if; 1:by auto.
+  by inline *; auto; call (: true); auto.
++ by proc; inline *; auto=> />.
++ by proc; inline *; auto=> />.
++ proc; rcondt {2} ^if; 1:by auto.
+  conseq (: ={glob Exp_b(SignedDH(S), RO), c})=> //.
+  by inline *; sim; auto.
++ proc; inline *; sp; if; auto.
+  conseq (: ={glob Exp_b(SignedDH(S), RO), k, c'})=> //.
+  sim; auto.
+  by call (: true); auto.
++ proc; sp; if; auto; sp; if; auto.
+  inline {1} 1.
+  conseq (: ={glob Exp_b(SignedDH(S), RO), ko})=> //.
+  by sim; auto.
++ conseq (: _ ==> ={glob RO, res})=> //.
+  proc *; inline {2} 1; rcondt {2} ^if; 1:by auto.
+  by sim.
+qed.
 
 (** Hop 1: Game 0 and Game 1 are equivalent (regardless of the value
     of the challenge bit) unless (and until) the gen oracle outputs a
@@ -885,77 +828,14 @@ local lemma Hop1 (b : bool) &m:
 (* This aborts the proof - we simply use the statement as a section heading. *)
 abort.
 
-(* In order to get the absolute values in, we need to make sure that
-   we can express the bad event on the left of the hop. While we do
-   this, we also set things up nicely to avoid having to reason about
-   equivalence up to bad in manual mode.
+(* This is an equivalence up to failure, which places some constraints
+   on the adversary, namely:
+   - that it cannot use non-termination as a behaviour to distinguish; and
+   - (later) that it cannot use the number of queries it makes as a
+     behaviour to distinguish.
+   The latter could be pushed into the proof; the former is not (yet?)
+   supported by the logics.
 *)
-local module Game05_b = {
-  include var Exp_b(SignedDH(S), RO, A) [-run]
-  include var Game1_b [-run]
-
-  module Oracles = {
-    (* The oracles are unchanged from Game1, except for gen *)
-    include Game1_b.Oracles [-gen]
-
-    proc gen(): pkey = {
-      var pk, sk;
-  
-      (pk, sk) <@ S.keygen();
-      if (has (fun i st=> st.`pk = pk /\ p_map.[i] = None) c_map) {
-        bad_1 <- true;
-        m <- m + 1;
-        pk_map.[m] <- pk;
-        sk_map.[m] <- sk;
-      } else {
-        m <- m + 1;
-        pk_map.[m] <- pk;
-        sk_map.[m] <- sk;
-      }
-      
-      return pk;
-    }
-  }
-
-  proc run(b) = {
-    var b';
-
-    RO.init();
-
-    b_ror <- b;
-
-    m <- 0;
-    n <- 0;
-
-    q <- fset0;
-    ich <- fset0;
-    rch <- fset0;
-    xp <- fset0;
-    cr <- fset0;
-
-    p_map <- empty;
-    i_map <- empty;
-    r_map <- empty;
-
-    pk_map <- empty;
-    sk_map <- empty;
-    c_map <- empty;
-
-    bad_1 <- false;
-    bad_2 <- false;
-
-    b' <@ A(Oracles).distinguish();
-    return b';
-  }
-}.
-
-(** Despite setting things up, the syntactic 'equivalent up to' tactic
-    is failing here for some reason. So we must do it by hand, which
-    requires us assuming that the adversary and the signature scheme
-    terminate.
-
-    This can pop off once the bugs in `byupto` are fixed.
-**)
 (* For all oracles that terminate, the adversary terminates *)
 declare axiom A_ll (O <: UATPaKE_RO_Oracles {-A}):
      islossless O.gen
@@ -971,28 +851,80 @@ declare axiom S_keygen_ll: islossless S.keygen.
 declare axiom S_sign_ll: islossless S.sign.
 declare axiom S_verify_ll: islossless S.verify.
 
+(* To get absolute values, we must make the event appear on the left *)
+local module Game05_b = {
+  include var Exp_b(SignedDH(S), RO, A) [-run]
+  include var Game0_b [-run]
+  include var Game1_b [-run]
+
+  module Oracles = {
+    include Game0_b.Oracles [-gen]
+
+    proc gen(): pkey = {
+      var sk, pk;
+ 
+      if (!halt_bad) {
+        m <- m + 1;
+        (pk, sk) <@ S.keygen();
+        pk_map.[m] <- pk;
+        sk_map.[m] <- sk;
+        if (has (fun i st=> st.`pk = pk /\ p_map.[i] = None) c_map) {
+          bad_1 <- true;
+        }
+      } else {
+        pk <- witness;
+      }
+      
+      return pk;
+    }
+  }
+
+  proc run(b) = {
+    var b';
+
+    RO.init();
+
+    halt_bad <- false;
+    b_ror <- b;
+
+    m <- 0;
+    n <- 0;
+
+    q <- fset0;
+    ich <- fset0;
+    rch <- fset0;
+    xp <- fset0;
+    cr <- fset0;
+
+    p_map <- empty;
+    i_map <- empty;
+    r_map <- empty;
+
+    pk_map <- empty;
+    sk_map <- empty;
+    c_map <- empty;
+
+    bad_1 <- false;
+    bad_2 <- false;
+
+    b' <@ A(Oracles).distinguish();
+    return b' /\ !halt_bad;
+  }
+}.
+
+local lemma Hop0_bad (b : bool) &m:
+  Pr[Game0_b.run(b) @ &m: res] = Pr[Game05_b.run(b) @ &m: res].
+proof.
+byequiv (: ={glob A, glob S, b} ==> ={res})=> //.
+by proc; sim.
+qed.
+
 local lemma Hop1 (b : bool) &m:
   `|Pr[Game0_b.run(b) @ &m: res] - Pr[Game1_b.run(b) @ &m: res]|
   <= Pr[Game1_b.run(b) @ &m: Game1_b.bad_1].
 proof.
-(* We need to make the bad event appear in the left game for the
-   absolute value to work out; this is just a pure equivalence
-   with a bit of a twist, since we modify *one* of the oracles
-   to branch on the failure event and set bad, but without changing
-   its obserable behaviour. The proof quickly focuses on this. *)
-have ->: Pr[Game0_b.run(b) @ &m: res] = Pr[Game05_b.run(b) @ &m: res].
-+ byequiv (: ={glob A, glob S, b} ==> ={res})=> //; proc.
-  call (: ={glob Exp_b, glob S, glob RO}); [2..7:by sim|8:by inline; auto].
-  by proc; auto; call (: true); auto=> />.
-(* Now, in theory, this could be done by the syntactic check: those
-   two games are syntactically equal except in branches that set bad
-   to true. However, this is borked right now, so we breathe in manual
-   mode, and we prove _semantically_ that:
-   1. Some invariant holds until bad happens, and implies the desired
-   equality of events in final memories;
-   2. Bad happens on both sides at the same time.
-*)
-byequiv: Game1_b.bad_1=> [||/#] //.
+rewrite Hop0_bad.
+byequiv (: ={glob A, glob S, b} ==> _): Game1_b.bad_1=> [||/#] //.
 proc.
 (* And now we lift the reasoning up to bad to the oracles the
    adversary has access to. Because we're in manual mode, and the
@@ -1005,20 +937,23 @@ proc.
    boolean variable), and that the state can be modified
    programmatically. It isn't some external, untouchable truth. *)
 call (: Game1_b.bad_1 (* the bad event *)
-      , ={glob Exp_b, glob S, glob RO, Game1_b.bad_1, Game1_b.bad_2} (* the invariant that holds until bad happens *)
-      , ={Game1_b.bad_1}). (* the invariant that holds after bad happens *)
+      (* The invariant that holds until bad happens *)
+      , ={glob Exp_b, glob S, glob RO, Game0_b.halt_bad, Game1_b.bad_1, Game1_b.bad_2}
+     /\ !Game0_b.halt_bad{2}
+      (* the invariant that holds after bad happens *)
+      , ={Game1_b.bad_1}).
 (* Goal 1: the adversary terminates if its oracles terminate. See above. *)
 + exact: A_ll.
 (* Goal i.0: if bad does not hold, and the non-bad invariant holds
    initially, then executing the oracles leads us to memories that are
    such that the correct invariant holds (depending on whether bad
    happened during the oracles' execution *)
-+ by proc; auto; call (: true); auto.
++ by proc; if; auto; call (: true); auto.
 (* Goal i.1: the left-hand side oracle terminates and preserves bad *)
-+ move=> &2 bad; proc; auto=> />.
-  by call S_keygen_ll; auto=> />; rewrite bad.
++ move=> &2 bad; proc; if; auto=> />.
+  by auto; call S_keygen_ll; auto=> />; rewrite bad.
 (* Goal i.2: the right-hand side oracle terminates and preserves bad *)
-+ move=> &1; proc; auto.
++ move=> &1; proc; if; auto.
   by call S_keygen_ll; auto=> />.
 (* Do those three again for all oracles *)
 + conseq (: ={glob Exp_b, glob S, glob RO, Game1_b.bad_1, Game1_b.bad_2, res})=> //.
@@ -1033,9 +968,9 @@ call (: Game1_b.bad_1 (* the bad event *)
 (* And again *)
 + conseq (: ={glob Exp_b, glob S, glob RO, Game1_b.bad_1, Game1_b.bad_2, res})=> //.
   by sim.
-+ move=> &2 bad; proc; auto=> /> &0.
++ move=> &2 bad; proc; if; auto=> /> &0.
   by rewrite dsk_ll /= /#.
-+ move=> &1; proc; auto=> /> &0.
++ move=> &1; proc; if; auto=> /> &0.
   by rewrite dsk_ll /= /#.
 (* And again *)
 + conseq (: ={glob Exp_b, glob S, glob RO, Game1_b.bad_1, Game1_b.bad_2, res})=> //.
@@ -1077,7 +1012,7 @@ admitted.
 local lemma Reduction1 b &m:
      B1.b_ror{m} = b
   => Pr[Game2_b.run(b) @ &m: Game1_b.bad_2]
-     <= Pr[SUFCMA(S, B1(S, A)).run() @ &m: res].
+     <= Pr[SUFCMA(S, B1(A)).run() @ &m: res].
 abort.
 
 (* We'd need to prove the same thing twice (once for each b) if we
@@ -1085,55 +1020,50 @@ abort.
    by going one level down.
 *)
 local equiv Reduction1_equiv:
-  Game2_b.run ~ SUFCMA(S, B1(S, A)).run:
+  Game2_b.run ~ SUFCMA(S, B1(A)).run:
        ={glob A, glob S, glob RO}
     /\ b{1} = B1.b_ror{2}
     ==> Game1_b.bad_2{1} => res{2}.
-(** HERE BE DRAGONS: we cannot immediately conclude that running
-    verification after the adversary returns (on the right) will
-    always give the same result as running it before the adversary's
-    run concludes (on the left). Here, we might just need to actually
-    halt and prevent the adversary to trigger more signing on the
-    left. (Or to restrict the class of signing algorithms the result
-    applies to, to a very reasonable class of algorithms where "if
-    verification succeeds once, then it succeeds every time on the
-    same input". This is slightly less reasonable if we want to allow
-    for stateful signature schemes...
-**)
+proof.
+(* Admit this for now---this is likely slightly less than true because
+   of the halting we have introduced in the games---we probably want
+   to make the reduction halt as well, but halting on bad_2 cannot
+   make the reduction fail (that is exactly the case where we have a
+   forgery available).
+   Everything here has to be so bespoke, it's like breathing in manual mode.
+*)
 admitted.
 
 local lemma Reduction1_0 &m:
   Pr[Game2_b.run(false) @ &m: Game1_b.bad_2]
-  <= Pr[SUFCMA(S, B1_0(S, A)).run() @ &m: res].
+  <= Pr[SUFCMA(S, B1_0(A)).run() @ &m: res].
 proof.
 byequiv (: ={glob A, glob S, glob RO} /\ !b{1} ==> Game1_b.bad_2{1} => res{2})=> //.
 proc *.
 transitivity {2}
   { B1.b_ror <- false;
-    r <@ SUFCMA(S, B1(S, A)).run(); }
+    r <@ SUFCMA(S, B1(A)).run(); }
   (={glob A, glob S, glob RO} /\ !b{1} ==> Game1_b.bad_2{1} => r{2})
   (={glob A, glob S, glob RO} ==> ={r})=> [/#|/>||].
 + by call Reduction1_equiv; auto=> />.
 + inline *; swap {2} 7 -6.
-  sim; wp=> />.
-  by sim: (={B1.forgery, b, SUFCMA.q, SUFCMA.cr, SUFCMA.pk_map, SUFCMA.n, glob S})=> />.
+  by sim.
 qed.
 
 local lemma Reduction1_1 &m:
   Pr[Game2_b.run(true) @ &m: Game1_b.bad_2]
-  <= Pr[SUFCMA(S, B1_1(S, A)).run() @ &m: res].
+  <= Pr[SUFCMA(S, B1_1(A)).run() @ &m: res].
 proof.
 byequiv (: ={glob A, glob S, glob RO} /\ b{1} ==> Game1_b.bad_2{1} => res{2})=> //.
 proc *.
 transitivity {2}
   { B1.b_ror <- true;
-    r <@ SUFCMA(S, B1(S, A)).run(); }
+    r <@ SUFCMA(S, B1(A)).run(); }
   (={glob A, glob S, glob RO} /\ b{1} ==> Game1_b.bad_2{1} => r{2})
   (={glob A, glob S, glob RO} ==> ={r})=> [/#|/>||].
 + by call Reduction1_equiv; auto=> />.
 + inline *; swap {2} 7 -6.
-  sim; wp=> />.
-  by sim: (={B1.forgery, b, SUFCMA.q, SUFCMA.cr, SUFCMA.pk_map, SUFCMA.n, glob S})=> />.
+  by sim.
 qed.
 
 local module Game3_b = {
@@ -1341,8 +1271,8 @@ local lemma Security_of_SignedDH &m:
     - Pr[Exp_b(SignedDH(S), RO, A).run(true) @ &m : res]|
   <=   Pr[Game1_b.run(true) @ &m: Game1_b.bad_1]
      + Pr[Game1_b.run(false) @ &m: Game1_b.bad_1]
-     + Pr[SUFCMA(S, B1_0(S, A)).run() @ &m: res]
-     + Pr[SUFCMA(S, B1_1(S, A)).run() @ &m: res]
+     + Pr[SUFCMA(S, B1_0(A)).run() @ &m: res]
+     + Pr[SUFCMA(S, B1_1(A)).run() @ &m: res]
      + 2%r * p
      + Pr[St_CDH(B2(S,A)).run() @ &m: res].
 proof.
